\documentclass[10pt]{article}
\usepackage{amsmath}
\usepackage{amssymb}
\usepackage{fullpage}

\DeclareMathOperator*{\argmin}{arg\,min}
\begin{document}

\begin{equation*}
    d(x,i)=E[Y^2 | X = x] +
    \sum_{j=1}^{N_Y} \sum_{k=1}^{N_X} \sum_{l=1}^{N_Y} ( {(x-x_{(k,l)})}^2 -
    2y_{(k,l)}E[Y|X=x,Y\in S_j] + y_{(k,l)}^2 )P(Y\in S_j|X=x)
    P(k,l|i,j)
\end{equation*}

\begin{equation*}
    d(y,j)=E[X^2 | Y = y] +
    \sum_{i=1}^{N_X} \sum_{k=1}^{N_X} \sum_{l=1}^{N_Y} ( {(y-y_{(k,l)})}^2 -
    2x_{(k,l)}E[X|Y=y,X\in R_i] + x_{(k,l)}^2 )P(X\in R_i|Y=y)
    P(k,l|i,j)
\end{equation*}

\begin{equation*}
    x_i = \argmin_x E[d(X,x)|X\in R_i]
\end{equation*}

The quantizer design algorithm is broken into two separate
stages\textemdash{}the initialization stage, followed by the channel
optimization stage. The purpose of the initialization stage is to initialize
the quantizer so a globally optimal average distortion can be achieved in the
channel optimization stage. In the initialization stage, we initialize the
quantizer according to a noiseless channel. In the channel optimization stage,
channel noise is slowly introduced while adjusting the codevectors and encoders
until the desired channel parameters are obtained.

\section*{Initialization Stage}
The following adaption of the LBG algorithm is used to initialize the quantizer.

\begin{enumerate}

    \item Apply uniform quantizer to training set $\mathcal{T}$. Let
        $q'_X(x):\mathbb{R} \rightarrow \{1,\ldots,L_X\}$
        and
        $q'_Y(y):\mathbb{R} \rightarrow \{1,\ldots,L_Y\}$
        denote the uniform quantizer functions for $X$ and $Y$ respectively and
        let $q_X(x'):\{1,\ldots,L_X\} \rightarrow \mathbb{R}$
        and
        $q_Y(y'):\{1,\ldots,L_Y\} \rightarrow \mathbb{R}$
        denote the reconstruction functions.

        For each $x'\in \{1,\ldots,L_X\}$, $y'\in \{1,\ldots,L_Y\}$ let
        \begin{equation*}
            m(x',y') = |\{(x,y) \in \mathcal{T} : q'_X(x) = x', q'_Y(y) = y'\}|
        \end{equation*}

    \item Let $N_X = 1$, $N_Y = 1$ and let
        \begin{align*}
            x_{(1,1)} &= \frac{1}{M}
            \sum_{x'=1}^{L_X} \sum_{y'=1}^{L_Y} q_X(x') m(x',y')
            \\
            y_{(1,1)} &= \frac{1}{M}
            \sum_{x'=1}^{L_X} \sum_{y'=1}^{L_Y} q_Y(y') m(x',y')
            \\
            D^*_{avg} &= \frac{1}{M} \sum_{x'=1}^{L_X} \sum_{y'=1}^{L_Y}
            \big( {(q_X(x')-x_{(1,1)})}^2 + {(q_Y(y')-y_{(1,1)})}^2 \big)
            m(x',y')
        \end{align*}

    \item Perform following splitting routine until desired value of $N_X$ is
        reached.
        \begin{enumerate}

            \item For each $i = 1,\ldots, N_X$, $j = 1,\ldots, N_Y$, let
                \begin{align*}
                    x_{(N_X+i,j)} &= (1+\epsilon)x_{(i,j)} \\
                    x_{(i,j)} &= (1-\epsilon)x_{(i,j)}
                \end{align*}
                for some small value of $\epsilon$.

            \item Let $N_X = 2N_X$.

            \item Let $D_{avg} = D^*_{avg}$

            \item For each $x'\in \{1,\ldots,L_X\}$ let 
                \begin{equation*}
                    I_X(x')=\argmin_{i \in \{1,\dots,N_X\}}d_X(x',i)
                \end{equation*}
                where
                \begin{equation*}
                    d_X(x',i) =
                    \frac{1}{M(x')} \bigg(T(x') + 
                    \sum_{j=1}^{N_Y}
                    \Big(\big({(q_X(x')-x_{(i,j)})}^2 +
                    y_{(i,j)}^2\big)M_j(x') -2y_{(i,j)}S_j(x')\Big)\bigg)
                \end{equation*}
                and
                \begin{align*}
                    M(x') &= {\sum_{y'=1}^{L_Y}m(x',y')} \\
                    M_j(x') &= \sum_{y':I_Y(y')=j}m(x',y') \\
                    S_j(x') &= \sum_{y':I_Y(y')=j}q_Y(y')m(x',y') \\
                    T(x') &= \sum_{y'=1}^{L_Y}{q_Y}^2(y')m(x',y')
                \end{align*}

            \item For each $k\in\{1,\ldots,N_X\}$, $l\in\{1,\ldots,N_Y\}$ let
                \begin{equation*}
                    x_{(i,j)} = 
                    \frac{\sum_{\substack{x':I_X(x')=i\\y':I_Y(y')=j}}q_X(x')m(x',y')}
                    {\sum_{\substack{x':I_X(x')=i\\y':I_Y(y')=j}}m(x',y')}
                \end{equation*}

            \item For each $y'\in \{1,\ldots,L_Y\}$ let 
                \begin{equation*}
                    I_Y(y')=\argmin_{j \in \{1,\dots,N_Y\}}d_Y(y',j)
                \end{equation*}
                where $d_Y(y',j)$ is defined in the same way as $d_X(x',i)$
                above.

            \item For each $k\in\{1,\ldots,N_X\}$, $l\in\{1,\ldots,N_Y\}$ let
                \begin{equation*}
                    y_{(i,j)} = 
                    \frac{\sum_{\substack{x':I_X(x')=i\\y':I_Y(y')=j}}q_Y(y')m(x',y')}
                    {\sum_{\substack{x':I_X(x')=i\\y':I_Y(y')=j}}m(x',y')}
                \end{equation*}

            \item Let 
                \begin{equation*}
                    D^*_{avg} = \frac{1}{M} \sum_{y'=1}^{L_Y}
                    d(y',I_Y(y')) \Big(\sum_{x'=1}^{L_X} m(x',y')\Big)
                \end{equation*}

            \item If
                $\frac
                {(D_{avg} - D^*_{avg})}
                {D_{avg}}
                > \delta$
                then return to step (c).
        \end{enumerate}

    \item Perform the same process as above for the $Y$ source until the
        desired value of $N_Y$ is reached.

\end{enumerate}

\section*{Channel Optimization Stage}

\begin{enumerate}
    \item For each $x'\in \{1,\ldots,L_X\}$ let 
        \begin{equation*}
            I_X(x')=\argmin_{i \in \{1,\dots,N_X\}}d_X(x',i)
        \end{equation*}
        where
        \begin{equation*}
            d_X(x',i) =
            \frac{1}{M(x')} \bigg(T(x') + 
            \sum_{j=1}^{N_Y} \sum_{k=1}^{N_X} \sum_{l=1}^{N_Y}
            \Big(\big({(q_X(x')-x_{(k,l)})}^2 +
            y_{(k,l)}^2\big)M_j(x') -2y_{(k,l)}S_j(x')\Big)P(k,l|i,j)\bigg)
        \end{equation*}
        and
        \begin{align*}
            M(x') &= {\sum_{y'=1}^{L_Y}m(x',y')} \\
            M_j(x') &= \sum_{y':I_Y(y')=j}m(x',y') \\
            S_j(x') &= \sum_{y':I_Y(y')=j}q_Y(y')m(x',y') \\
            T(x') &= \sum_{y'=1}^{L_Y}{q_Y}^2(y')m(x',y')
        \end{align*}
    \item For each $k\in\{1,\ldots,N_X\}$, $l\in\{1,\ldots,N_Y\}$ let
        \begin{equation*}
            x_{(k,l)} = 
            \frac{\sum_{i=1}^{N_X} \sum_{j=1}^{N_Y}
            S_{(i,j)}^X P(k,l|i,j)}
            {\sum_{i=1}^{N_X} \sum_{j=1}^{N_Y}
            M_{(i,j)} P(k,l|i,j)}
        \end{equation*}
        where
        \begin{align*}
            M_{(i,j)} &=
            \sum_{\substack{x':I_X(x')=i\\y':I_Y(y')=j}}m(x',y') \\
            S^X_{(i,j)} &=
            \sum_{\substack{x':I_X(x')=i\\y':I_Y(y')=j}}q(x')m(x',y')
        \end{align*}
\end{enumerate}
\end{document}

